fstar/glue/proofs/MLS.NetworkBinder.Properties.Proofs.fst
@@ -1,0 +1,180 @@
+module MLS.NetworkBinder.Properties.Proofs
+
+open Comparse
+open MLS.Crypto
+open MLS.TreeSync.NetworkTypes
+open MLS.TreeKEM.NetworkTypes
+open MLS.NetworkBinder
+open MLS.NetworkBinder.Properties
+open MLS.Tree
+open MLS.TreeCommon
+open MLS.Result
+open MLS.MiscLemmas
+
+#set-options "--fuel 1 --ifuel 1"
+
+(*** Path filtering invariants ***)
+
+val path_filtering_ok_uncompress_update_path_aux:
+  #bytes:Type0 -> {|bytes_like bytes|} ->
+  #leaf_t:Type -> #node_t:Type ->
+  #l:nat -> #i:tree_index l ->
+  li:leaf_index l i -> t:tree (option leaf_t) (option node_t) l i -> leaf_node:leaf_node_nt bytes tkt -> nodes:list (update_path_node_nt bytes) ->
+  Lemma (
+    match uncompress_update_path_aux li t (leaf_node, nodes) with
+    | Success res -> path_filtering_ok t res
+    | _ -> True
+  )
+let rec path_filtering_ok_uncompress_update_path_aux #bytes #bl #leaf_t #node_t #l #i li t leaf_node nodes =
+  match t with
+  | TLeaf _ -> (
+    if not (List.length nodes = 0) then ()
+    else ()
+  )
+  | TNode _ left right -> (
+    let (child, sibling) = get_child_sibling t li in
+    if is_tree_empty sibling then (
+      path_filtering_ok_uncompress_update_path_aux (li <: leaf_index (l-1) _) child leaf_node nodes
+    ) else (
+      if not (List.length nodes > 0) then ()
+      else (
+        let (tail_nodes, head_nodes) = List.unsnoc nodes in
+        path_filtering_ok_uncompress_update_path_aux (li <: leaf_index (l-1) _) child leaf_node tail_nodes
+      )
+    )
+  )
+
+val path_filtering_ok_uncompress_update_path:
+  #bytes:Type0 -> {|bytes_like bytes|} ->
+  #leaf_t:Type -> #node_t:Type ->
+  #l:nat -> #i:tree_index l ->
+  li:leaf_index l i -> t:tree (option leaf_t) (option node_t) l i -> update_path:update_path_nt bytes ->
+  Lemma (
+    match uncompress_update_path li t update_path with
+    | Success res -> path_filtering_ok t res
+    | _ -> True
+  )
+let path_filtering_ok_uncompress_update_path #bytes #bl #leaf_t #node_t #l #i li t update_path =
+  path_filtering_ok_uncompress_update_path_aux li t update_path.leaf_node update_path.nodes
+
+val path_filtering_ok_update_path_to_treesync:
+  #bytes:Type0 -> {|crypto_bytes bytes|} ->
+  #leaf_t:Type -> #node_t:Type ->
+  #l:nat -> #i:tree_index l -> #li:leaf_index l i ->
+  t:tree (option leaf_t) (option node_t) l i ->
+  p:sparse_update_path bytes l i li ->
+  Lemma
+  (requires path_filtering_ok t p)
+  (ensures path_filtering_ok t (update_path_to_treesync p))
+let rec path_filtering_ok_update_path_to_treesync #bytes #cb #leaf_t #node_t #l #i #li t p =
+  match p with
+  | PLeaf ln -> ()
+  | PNode onp p_next -> (
+    let (child, _) = get_child_sibling t li in
+    path_filtering_ok_update_path_to_treesync child p_next
+  )
+
+val path_filtering_ok_set_path_leaf:
+  #tree_leaf_t:Type -> #tree_node_t:Type ->
+  #path_in_leaf_t:Type -> #path_out_leaf_t:Type -> #path_node_t:Type ->
+  #l:nat -> #i:tree_index l -> #li:leaf_index l i ->
+  t:tree (option tree_leaf_t) (option tree_node_t) l i ->
+  p:path path_in_leaf_t (option path_node_t) l i li -> lp:path_out_leaf_t ->
+  Lemma
+  (requires path_filtering_ok t p)
+  (ensures path_filtering_ok t (set_path_leaf p lp))
+let rec path_filtering_ok_set_path_leaf #tree_leaf_t #tree_node_t #path_in_leaf_t #path_out_leaf_t #path_node_t #l #i #li t p lp =
+  match p with
+  | PLeaf _ -> ()
+  | PNode _ p_next -> (
+    let (child, _) = get_child_sibling t li in
+    path_filtering_ok_set_path_leaf child p_next lp
+  )
+
+val path_filtering_ok_update_path_to_treekem:
+  #bytes:Type0 -> {|crypto_bytes bytes|} ->
+  #tree_leaf_t:Type -> #tree_node_t:Type ->
+  #l:nat -> #i:tree_index l -> #li:leaf_index l i ->
+  t:tree (option tree_leaf_t) (option tree_node_t) l i ->
+  p:sparse_update_path bytes l i li ->
+  Lemma
+  (requires path_filtering_ok t p)
+  (ensures path_filtering_ok t (update_path_to_treekem p))
+let path_filtering_ok_update_path_to_treekem #bytes #cb #tree_leaf_t #tree_node_t #l #i #li t p =
+  path_filtering_ok_set_path_leaf t p (leaf_node_to_treekem (get_path_leaf p))
+
+(*** Correctness of compression / decompression ***)
+
+val compress_uncompress_update_path_aux:
+  #bytes:Type0 -> {|bytes_like bytes|} ->
+  #leaf_t:Type -> #node_t:Type ->
+  #l:nat -> #i:tree_index l ->
+  li:leaf_index l i -> t:tree (option leaf_t) (option node_t) l i -> update_path:(leaf_node_nt bytes tkt & list (update_path_node_nt bytes)) ->
+  Lemma (
+    match uncompress_update_path_aux li t update_path with
+    | Success p -> compress_update_path_aux p == update_path
+    | _ -> True
+  )
+let rec compress_uncompress_update_path_aux #bytes #bl #leaf_t #node_t #l #i li t (leaf_node, nodes) =
+  match t with
+  | TLeaf _ -> (
+    if not (List.length nodes = 0) then ()
+    else ()
+  )
+  | TNode _ left right -> (
+    let (child, sibling) = get_child_sibling t li in
+    if is_tree_empty sibling then (
+      compress_uncompress_update_path_aux (li <: leaf_index (l-1) _) child (leaf_node, nodes)
+    ) else (
+      if not (List.length nodes > 0) then ()
+      else (
+        let (tail_nodes, head_nodes) = List.unsnoc nodes in
+        compress_uncompress_update_path_aux (li <: leaf_index (l-1) _) child (leaf_node, tail_nodes)
+      )
+    )
+  )
+
+val compress_uncompress_update_path:
+  #bytes:Type0 -> {|bytes_like bytes|} ->
+  #leaf_t:Type -> #node_t:Type ->
+  #l:nat -> #i:tree_index l ->
+  li:leaf_index l i -> t:tree (option leaf_t) (option node_t) l i -> update_path:update_path_nt bytes ->
+  Lemma (
+    match uncompress_update_path li t update_path with
+    | Success p -> compress_update_path p == Success update_path
+    | _ -> True
+  )
+let compress_uncompress_update_path #bytes #bl #leaf_t #node_t #l #i li t update_path =
+  compress_uncompress_update_path_aux li t (update_path.leaf_node, update_path.nodes)
+
+val uncompress_compress_update_path_aux:
+  #bytes:Type0 -> {|bytes_like bytes|} ->
+  #leaf_t:Type -> #node_t:Type ->
+  #l:nat -> #i:tree_index l -> #li:leaf_index l i ->
+  t:tree (option leaf_t) (option node_t) l i ->
+  p:sparse_update_path bytes l i li ->
+  Lemma
+  (requires path_filtering_ok t p)
+  (ensures uncompress_update_path_aux li t (compress_update_path_aux p) == Success p)
+let rec uncompress_compress_update_path_aux #bytes #bl #leaf_t #node_t #l #i #li t p =
+  match p with
+  | PLeaf ln -> ()
+  | PNode p_opt_data p_next ->
+    let (child, _) = get_child_sibling t li in
+    uncompress_compress_update_path_aux child p_next
+
+val uncompress_compress_update_path:
+  #bytes:Type0 -> {|bytes_like bytes|} ->
+  #leaf_t:Type -> #node_t:Type ->
+  #l:nat -> #i:tree_index l -> #li:leaf_index l i ->
+  t:tree (option leaf_t) (option node_t) l i ->
+  p:sparse_update_path bytes l i li ->
+  Lemma
+  (requires path_filtering_ok t p)
+  (ensures (
+    match compress_update_path p with
+    | Success update_path -> uncompress_update_path li t update_path == Success p
+    | _ -> True
+  ))
+let uncompress_compress_update_path #bytes #bl #leaf_t #node_t #l #i #li t p =
+  uncompress_compress_update_path_aux t p
